theories/utp_common.thy
@@ -206,7 +206,7 @@ text {* Ad-hoc overloading allows the binding of symbols to multiple
 
 consts
   alphabet     :: "'r \<Rightarrow> 'a" ("\<alpha>")
-  alpha_coerce :: "'p \<Rightarrow> 'a \<Rightarrow> 'q" ("_\<^bsub>!_\<^esub>")
+  alpha_coerce :: "'p \<Rightarrow> 'a \<Rightarrow> 'q" ("_\<^bsub>!_\<^esub>" [1000,0] 1000)
   prime        :: "'a \<Rightarrow> 'a" ("_\<acute>" [1000] 1000)
   unprime      :: "'a \<Rightarrow> 'a" ("_~" [1000] 1000)
   subscr       :: "'a \<Rightarrow> nat \<Rightarrow> 'a" ("_\<^bsub>_\<^esub>")
